Cleaning up

Properties.v
@@ -16,15 +16,15 @@ Ltac splits n :=
 (* Determinism ------------------------------------------------------------- *)
 (* ------------------------------------------------------------------------- *)
 
-Lemma value_does_not_step : forall m m' v t eff,
-  value v -> ~ (m / v --> eff / m' / t).
+Lemma value_does_not_step : forall v eff t,
+  value v -> ~ (v --[eff]--> t).
 Proof.
   intros * Hv Hstep. destruct Hv; inversion Hstep.
 Qed.
 
-Theorem deterministic_step : forall m m' t t1 t2 eff,
-  m / t --> eff / m' / t1 ->
-  m / t --> eff / m' / t2 ->
+Theorem deterministic_step : forall t eff t1 t2,
+  t --[eff]--> t1 ->
+  t --[eff]--> t2 ->
   t1 = t2.
 Proof.
   intros * Hstep1. generalize dependent t2.
@@ -32,14 +32,14 @@ Proof.
   try solve
     [ congruence
     | match goal with
-      | Hstep : _ / ?v --> _ / _ / _ , Hv : value ?v |- _ =>
-        exfalso; apply (value_does_not_step _ _ _ _ _ Hv Hstep); auto
-      | F : _ / TM_Nil         --> _ / _ / _ |- _ => inversion F
-      | F : _ / TM_Num _       --> _ / _ / _ |- _ => inversion F
-      | F : _ / TM_Arr _ _     --> _ / _ / _ |- _ => inversion F
-      | F : _ / TM_Fun _ _ _ _ --> _ / _ / _ |- _ => inversion F
-      | F : _ / TM_Loc _       --> _ / _ / _ |- _ => inversion F
-      | H : forall x, _ / _ --> _ / _ / x -> _ = x |- _ => erewrite H; eauto
+      | Hstep : ?v --[ _ ]--> _ , Hv : value ?v |- _ =>
+          eapply value_does_not_step in Hstep; eauto; contradiction
+      | F : TM_Nil         --[ _ ]--> _ |- _ => inversion F
+      | F : TM_Num _       --[ _ ]--> _ |- _ => inversion F
+      | F : TM_Arr _ _     --[ _ ]--> _ |- _ => inversion F
+      | F : TM_Fun _ _ _ _ --[ _ ]--> _ |- _ => inversion F
+      | F : TM_Loc _       --[ _ ]--> _ |- _ => inversion F
+      | H : forall x, _ --[ _ ]--> x -> _ = x |- _ => erewrite H; eauto
       end
     ].
 Qed.
@@ -63,12 +63,22 @@ Proof.
 Qed.
 
 (* ------------------------------------------------------------------------- *)
-(* Progress, Preservation & Soundness -------------------------------------- *)
+(* Definitions ------------------------------------------------------------- *)
 (* ------------------------------------------------------------------------- *)
 
-Definition well_typed_memory (mt : list typ) (m : mem) :=
+Definition well_typed_memory mt m :=
   length mt = length m /\
   (forall i, mt / empty |-- (get_tm m i) is (get_typ mt i)).
+
+Definition well_typed_threads mt ths := forall i,
+  exists T, mt / empty |-- (get_tm ths i) is T.
+
+Definition well_typed_program mt m ths :=
+  well_typed_memory mt m /\
+  well_typed_threads mt ths.
+
+Definition finished ths :=
+  forall i, value (get_tm ths i).
 
 Inductive extends' {A} : list A -> list A -> Prop :=
   | extends_nil : forall mt,
@@ -79,14 +89,40 @@ Inductive extends' {A} : list A -> list A -> Prop :=
 
 Infix "extends" := extends' (at level 50, left associativity).
 
-Lemma extends_lookup : forall i (mt mt' : list typ),
+(* ------------------------------------------------------------------------- *)
+(* Auxiliary Lemmas -------------------------------------------------------- *)
+(* ------------------------------------------------------------------------- *)
+
+Lemma extends_refl : forall {A} (mt : list A),
+  mt extends mt.
+Proof.
+  induction mt; auto using @extends'.
+Qed.
+
+Lemma extends_add : forall {A} (mt : list A) a,
+  (add mt a) extends mt.
+Proof.
+  induction mt; eauto using @extends'.
+Qed.
+
+Lemma extends_length : forall {A} (mt mt' : list A) i,
+  i < length mt' ->
+  mt extends mt' ->
+  i < length mt.
+Proof.
+  intros *. generalize dependent mt. generalize dependent i.
+  induction mt'; intros * Hlen Hext.
+  - inversion Hlen.
+  - inversion Hext. destruct i;
+    eauto using PeanoNat.Nat.lt_0_succ, Lt.lt_n_S, Lt.lt_S_n.
+Qed.
+
+Lemma extends_lookup : forall (mt mt' : list typ) i,
   i < length mt' ->
   mt extends mt' ->
   get_typ mt' i = get_typ mt i.
 Proof.
-  intros *.
-  generalize dependent mt.
-  generalize dependent i.
+  intros *. generalize dependent mt. generalize dependent i.
   induction mt'; intros * Hlen Hext.
   - inversion Hlen.
   - inversion Hext. subst. destruct i.
@@ -94,30 +130,24 @@ Proof.
     + unfold get_typ, get. simpl in *. eauto using Lt.lt_S_n.
 Qed.
 
-Lemma extends_length : forall {A} i (mt mt' : list A),
-  i < length mt' ->
-  mt extends mt' ->
-  i < length mt.
+Lemma safe_preserves_inclusion : forall Gamma Gamma',
+  Gamma includes Gamma' ->
+  (safe Gamma) includes (safe Gamma').
 Proof.
-  intros *.
-  generalize dependent mt.
-  generalize dependent i.
-  induction mt'; intros * Hlen Hext.
-  - inversion Hlen.
-  - inversion Hext. destruct i;
-    eauto using PeanoNat.Nat.lt_0_succ, Lt.lt_n_S, Lt.lt_S_n.
+  unfold Map.includes', safe. intros * H *.
+  destruct (Gamma k) eqn:E1; destruct (Gamma' k) eqn:E2;
+  solve [ intros F; inversion F
+        | eapply H in E2; rewrite E1 in E2; inversion E2; subst; trivial
+        ].
 Qed.
 
-Lemma extends_add : forall {A} (mt : list A) x,
-  (add mt x) extends mt.
+Lemma update_safe_includes_safe_update : forall Gamma id T,
+  (update (safe Gamma) id T) includes (safe (update Gamma id T)).
 Proof.
-  induction mt; eauto using @extends'.
-Qed.
-
-Lemma extends_refl : forall {A} (mt : list A),
-  mt extends mt.
-Proof.
-  induction mt; auto using @extends'.
+  unfold Map.includes', update, Map.update', safe. intros *.
+  destruct String.eqb; trivial.
+  destruct is_safe_type; trivial.
+  intros F. inversion F.
 Qed.
 
 Lemma memory_weakening : forall mt mt' Gamma t T, 
@@ -130,16 +160,14 @@ Proof.
   subst; erewrite extends_lookup; eauto using extends_length, @typeof.
 Qed.
 
-Lemma safe_preserves_inclusion : forall Gamma Gamma',
-  Gamma includes Gamma' ->
-  (safe Gamma) includes (safe Gamma').
+Lemma concurrent_memory_weakening : forall mt mt' ths,
+  mt' extends mt ->
+  well_typed_threads mt ths ->
+  well_typed_threads mt' ths.
 Proof.
-  unfold Map.includes', safe. intros * H *.
-  destruct (Gamma k) eqn:E1; destruct (Gamma' k) eqn:E2;
-  solve 
-    [ intros F; inversion F
-    | eapply H in E2; rewrite E1 in E2; inversion E2; subst; trivial
-    ].
+  intros * Hext Hths. intros i.
+  specialize (Hths i) as [? ?]. eexists.
+  eauto using memory_weakening.
 Qed.
 
 Lemma context_weakening : forall mt Gamma Gamma' t T,
@@ -160,30 +188,6 @@ Proof.
   intros * Htype.
   eapply (context_weakening _ _ empty); auto.
   discriminate.
-Qed.
-
-Lemma assignment_preserves_memory_typing : forall m mt t i,
-  i < length m ->
-  well_typed_memory mt m ->
-  mt / empty |-- t is (get_typ mt i) ->
-  well_typed_memory mt (set m i t).
-Proof.
-  intros * Hi [Hlen Htype1] Htype2. split.
-  - rewrite Hlen. apply set_preserves_length.
-  - intros j. destruct (PeanoNat.Nat.eqb i j) eqn:E.
-    + apply PeanoNat.Nat.eqb_eq in E. subst.
-      erewrite (get_set_involutive TM_Nil); auto.
-    + apply PeanoNat.Nat.eqb_neq in E. subst.
-      erewrite (get_set_i_neq_j TM_Nil); auto.
-Qed.
-
-Lemma update_safe_includes_safe_update : forall Gamma id T,
-  (update (safe Gamma) id T) includes (safe (update Gamma id T)).
-Proof.
-  unfold Map.includes', update, Map.update', safe. intros *.
-  destruct String.eqb; trivial.
-  destruct is_safe_type; trivial.
-  intros F. inversion F.
 Qed.
 
 Lemma substitution_preserves_typing : forall mt Gamma id t u T U,
@@ -216,13 +220,62 @@ Proof with eauto using context_weakening, context_weakening_empty,
   - apply T_Fun...
 Qed.
 
-Lemma add_preserves_well_typed_memories : forall mt m t T,
+Lemma alloc_value_has_type : forall mt t t' addr v T,
+  mt / empty |-- t is T ->
+  t --[EF_Alloc addr v]--> t' ->
+  exists V, mt / empty |-- v is V.
+Proof.
+  remember empty as Gamma.
+  intros * Htype. generalize dependent t'.
+  induction Htype; intros * Hstep; inversion Hstep; subst; eauto.
+Qed.
+
+Lemma store_value_has_type : forall mt t t' addr v T,
+  mt / empty |-- t is T ->
+  t --[EF_Store addr v]--> t' ->
+  mt / empty |-- v is (get_typ mt addr).
+Proof.
+  remember empty as Gamma.
+  intros * Htype. generalize dependent t'.
+  induction Htype; intros * Hstep;
+  inversion Hstep; subst; eauto;
+  solve [match goal with
+    | H1 : _ / _ |-- ?v is _,
+      H2 : _ / _ |-- _  is _
+      |- _ / _ |-- ?v is _ =>
+        inversion H2; subst; eauto
+    end].
+Qed.
+
+Lemma spawn_block_has_type : forall mt t t' block T,
+  mt / empty |-- t is T ->
+  t --[EF_Spawn block]--> t' ->
+  exists B, mt / empty |-- block is B.
+Proof.
+  remember empty as Gamma.
+  intros * Htype. generalize dependent t'.
+  induction Htype; intros * Hstep; inversion Hstep; subst; eauto.
+Qed.
+
+Lemma store_preserves_well_typed_memory : forall m mt t i,
+  i < length m ->
+  well_typed_memory mt m ->
+  mt / empty |-- t is (get_typ mt i) ->
+  well_typed_memory mt (set m i t).
+Proof.
+  intros * ? [Hlen ?] ?. split.
+  - rewrite Hlen. apply set_preserves_length.
+  - intros j. destruct (i =? j) eqn:E.
+    + apply Nat.eqb_eq in E. subst. erewrite (get_i_set_i TM_Nil); auto.
+    + apply Nat.eqb_neq in E. erewrite (get_i_set_j TM_Nil); auto.
+Qed.
+
+Lemma alloc_preserves_well_typed_memory : forall mt m t T,
   well_typed_memory mt m ->
   mt / empty |-- t is T ->
   well_typed_memory (add mt T) (add m t).
 Proof.
-  intros * [Hlen H] Htype.
-  unfold well_typed_memory.
+  intros * [Hlen Hmem] Htype.
   split; auto using add_preserves_length. intros i.
   destruct (lt_eq_lt_dec i (length m)) as [[Hlt | Heq] | Hgt];
   unfold get_tm, get_typ in *; subst.
@@ -238,285 +291,253 @@ Proof.
     apply T_Nil.
 Qed.
 
-Theorem preservation : forall m m' mt t t' eff T,
+Lemma step_preserves_well_typed_threads : forall mt ths t T i,
+  i < length ths ->
+  well_typed_threads mt ths ->
   mt / empty |-- t is T ->
-  well_typed_memory mt m ->
-  m / t --> eff / m' / t' ->
-  exists mt',
-    mt' extends mt /\
-    mt' / empty |-- t' is T /\
-    well_typed_memory mt' m'.
+  well_typed_threads mt (set ths i t).
 Proof.
-  remember empty as Gamma.
-  intros * Htype.
-  generalize dependent t'.
-  induction Htype;
-  intros * Hmem Hstep;
-  inversion Hstep; subst;
-  try solve
-    [ match goal with
-      | IH : _ -> _ -> _ -> _ -> exists mt', _ /\ _ /\ _,
-        H  : _ / _ --> _ / _ / _ |- _ =>
-          eapply IH in H; trivial; destruct H as [? [? [? ?]]];
-          eexists; splits 3; eauto using memory_weakening, @typeof
-      end
-    | exists mt; splits 3; eauto using extends_refl, @typeof;
-      match goal with H : _ / _ |-- _ is _ |- _ =>
-        inversion H; subst;
-        solve [ destruct Hmem; trivial
-              | auto using assignment_preserves_memory_typing
-              | eauto using substitution_preserves_typing
-              ]
-      end
-    | exists (add mt E); inversion Hmem as [Hlen ?]; rewrite <- Hlen;
-      splits 3; auto using extends_add, add_preserves_well_typed_memories;
-      eauto using @typeof, length_l_lt_add, get_add_last
-    ].
-  (* LetVar *)
-  - exists (add mt E). inversion Hmem as [Hlen ?]. rewrite <- Hlen.
-    splits 3; auto using extends_add, add_preserves_well_typed_memories.
-    eapply substitution_preserves_typing;
-    eauto using extends_add, memory_weakening.
-    assert (Haux : TY_Ref E = TY_Ref (get_typ (add mt E) (length mt))).
-    { unfold get_typ. rewrite (get_add_last TY_Void). reflexivity. }
-    rewrite Haux. auto using T_Loc, length_l_lt_add.
+  intros * Hlen Htype Hstep.
+  intros i'. destruct (i =? i') eqn:E.
+  - apply Nat.eqb_eq in E. subst.
+    rewrite (get_i_set_i TM_Nil); eauto.
+  - apply Nat.eqb_neq in E. apply not_eq_sym in E.
+    rewrite (get_i_set_j TM_Nil); eauto.
 Qed.
 
-Theorem progress : forall m mt t T,
+Lemma spawn_preserves_well_typed_threads : forall mt ths t T,
+  well_typed_threads mt ths ->
   mt / empty |-- t is T ->
-  well_typed_memory mt m ->
-  (value t \/ exists m' t' eff, m / t --> eff / m' / t').
+  well_typed_threads mt (add ths t).
 Proof.
-  remember empty as Gamma. intros * Htype [Hlen Hmem].
-  assert (forall i, i < length mt -> i < length m). { rewrite Hlen. trivial. }
+  intros * Hths Htype.
+  intros i. destruct (lt_eq_lt_dec i (length ths)) as [[? | Heq] | Hlt].
+  - specialize (Hths i) as [? ?]. rewrite (get_add_lt TM_Nil); eauto.
+  - subst. rewrite (get_add_last TM_Nil). eauto.
+  - rewrite (get_add_gt TM_Nil); eauto using T_Nil.
+Qed.
+
+Definition is_alloc_or_load eff :=
+  match eff with
+  | EF_Alloc _ _ | EF_Load _ _ => true
+  | _ => false
+  end.
+
+Lemma limited_preservation : forall mt m t t' eff T,
+  well_typed_memory mt m ->
+  mt / empty |-- t is T ->
+  t --[eff]--> t' ->
+  is_alloc_or_load eff = false ->
+  mt / empty |-- t' is T.
+Proof.
+  remember empty as Gamma.
+  intros * [Hlen Hmem] Htype Hstep Heff.
+  generalize dependent t'.
+  induction Htype; intros * Hstep; inversion Hstep; subst;
+  try solve [ discriminate Heff
+            | eauto using substitution_preserves_typing, @typeof
+            ].
+  - match goal with
+    | Htype : _ / _ |-- _ is TY_Fun _ _ |- _ => inversion Htype; subst
+    end.
+    eauto using substitution_preserves_typing.
+Qed.
+
+Lemma alloc_preservation : forall mt t t' v T V,
+  mt / empty |-- t is T ->
+  mt / empty |-- v is V ->
+  t --[EF_Alloc (length mt) v]--> t' ->
+  (add mt V) / empty |-- t' is T.
+Proof.
+  remember empty as Gamma.
+  intros * Htype ? Hstep. generalize dependent t'.
+  assert (R : forall T, T = get_typ (add mt T) (length mt)).
+  { intros. eauto using get_add_last. }
+  induction Htype; intros * Hstep; inversion Hstep; subst;
+  eauto using @typeof, extends_add, memory_weakening;
+  match goal with
+  | H1 : mt / _ |-- v is ?T1, H2 : mt / _ |-- v is ?T2 |- _ =>
+    eapply (deterministic_typing _ _ _ T1 T2) in H1; eauto; subst
+  end;
+  try match goal with
+  |- _ / _ |-- _ is _ ?T =>
+    rewrite (R T); eauto using @typeof, length_lt_add
+  end.
+  - eapply substitution_preserves_typing;
+    eauto using extends_add, memory_weakening.
+    assert (R' : forall T, TY_Ref T = TY_Ref (get_typ (add mt T) (length mt))).
+    { intros. f_equal. eauto using get_add_last. }
+    rewrite R'. eauto using @typeof, length_lt_add.
+Qed.
+
+Lemma load_preservation : forall mt m t t' addr T,
+  well_typed_memory mt m ->
+  mt / empty |-- t is T ->
+  t --[EF_Load addr (get_tm m addr)]--> t' ->
+  mt / empty |-- t' is T.
+Proof.
+  remember empty as Gamma.
+  intros * [Hlen Hmem] Htype Hstep. generalize dependent t'.
+  induction Htype; intros * Hstep; inversion Hstep; subst;
+  try solve [ eauto using @typeof
+            | repeat match goal with 
+              | H : _ / _ |-- _ is _ |- _ => inversion H; subst; eauto
+              end
+            ].
+Qed.
+
+(* ------------------------------------------------------------------------- *)
+(* Preservation ------------------------------------------------------------ *)
+(* ------------------------------------------------------------------------- *)
+
+Theorem preservation : forall mt m m' ths ths' ceff,
+  well_typed_program mt m ths ->
+  m / ths ==> m' / ths' # ceff ->
+  exists mt',
+    mt' extends mt /\
+    well_typed_program mt' m' ths'.
+Proof.
+  intros * [Hmem Hths] Hcstep.
+  inversion Hcstep; subst; destruct (Hths i) as [? ?].
+  (* None *)
+  - eexists. splits 3; eauto using extends_refl.
+    intros i'. destruct (i =? i') eqn:E.
+    + apply Nat.eqb_eq in E. subst.
+      rewrite (get_i_set_i TM_Nil); trivial.
+      specialize (Hths i') as [? ?]. eexists.
+      eauto using limited_preservation.
+    + apply Nat.eqb_neq in E. apply not_eq_sym in E.
+      rewrite (get_i_set_j TM_Nil); trivial.
+  (* Alloc *)
+  - rewrite <- (proj1 Hmem) in *.
+    assert (exists V, mt / empty |-- v is V) as [V ?].
+    { eauto using alloc_value_has_type. }
+    exists (add mt V). splits 3;
+    eauto using extends_add,
+      alloc_preserves_well_typed_memory,
+      step_preserves_well_typed_threads,
+      concurrent_memory_weakening,
+      alloc_preservation.
+  (* Load *)
+  - eexists. splits 3; eauto using extends_refl.
+    eauto using step_preserves_well_typed_threads, load_preservation.
+  (* Store *)
+  - eexists. splits 3; eauto using extends_refl;
+    eauto using store_preserves_well_typed_memory,
+      store_value_has_type,
+      step_preserves_well_typed_threads,
+      limited_preservation.
+  (* Spawn *)
+  - eexists. splits 3; eauto using extends_refl.
+    assert (exists B, mt / empty |-- block is B) as [? ?].
+    { eauto using spawn_block_has_type. }
+    eauto using spawn_preserves_well_typed_threads,
+      step_preserves_well_typed_threads,
+      limited_preservation.
+Qed.
+
+(* ------------------------------------------------------------------------- *)
+(* Progress ---------------------------------------------------------------- *)
+(* ------------------------------------------------------------------------- *)
+
+Lemma well_typed_threads_tail : forall mt th ths,
+  well_typed_threads mt (th :: ths) ->
+  well_typed_threads mt ths.
+Proof.
+  intros * Hths. intros i.
+  specialize (Hths (S i)) as [T Htype].
+  eexists. eauto.
+Qed.
+
+Lemma concurrent_step_weakening : forall m m' th ths ths' ceff,
+  m / ths ==> m' / ths' # ceff ->
+  exists ceff', m / (th :: ths) ==> m' / (th :: ths') # ceff'.
+Proof.
+  intros * Hcstep.
+  inversion Hcstep; subst;
+  solve [rewrite set_tail || rewrite add_set_tail; eauto using cstep, lt_n_S].
+Qed.
+
+Inductive well_behaved_effect : effect -> mem -> Prop :=
+  | WBE_None : forall m,
+    well_behaved_effect EF_None m
+
+  | WBE_Spawn : forall m block,
+    well_behaved_effect (EF_Spawn block) m
+
+  | WBE_Alloc : forall m v,
+    well_behaved_effect (EF_Alloc (length m) v) m
+
+  | WBE_Load : forall m addr,
+    well_behaved_effect (EF_Load addr (get_tm m addr)) m
+
+  | WBE_Store : forall m addr v,
+    addr < length m ->
+    well_behaved_effect (EF_Store addr v) m
+  .
+
+Lemma memory_length : forall mt m i,
+  well_typed_memory mt m ->
+  (i < length mt) -> (i < length m).
+Proof.
+  intros * [Hlen _]. rewrite Hlen. trivial.
+Qed.
+
+Lemma limited_progress : forall mt m t T,
+  well_typed_memory mt m ->
+  mt / empty |-- t is T ->
+  value t \/ exists t' eff',
+    t --[eff']--> t' /\
+    well_behaved_effect eff' m.
+Proof.
+  remember empty as Gamma.
+  intros * Hmem Htype.
   induction Htype; subst; auto using value; right;
   try match goal with F : lookup empty _ = Some _ |- _ => inversion F end;
   repeat match goal with
-    IH : _ = empty -> _ |- _ => specialize (IH eq_refl) as [? | [? [? [? ?]]]]
+    IH : _ -> _ \/ _ |- _ => specialize (IH eq_refl) as [? | [? [? [? ?]]]]
   end;
-  try solve [eexists; eexists; eexists; eauto using step];
+  try solve [eexists; eexists; split; eauto using step, well_behaved_effect];
   repeat match goal with
     Hv : value ?t , Htype : _ / _ |-- ?t is _ |- _ =>
       destruct Hv; inversion Htype; subst
   end;
-  eexists; eexists; eexists; eauto using step, value.
+  eexists; eexists; split;
+  eauto using memory_length, step, value, well_behaved_effect.
 Qed.
 
-Definition normal_form m t : Prop :=
-  ~ exists m' t' eff, m / t --> eff / m' / t'.
-
-Definition stuck m t : Prop := normal_form m t /\ ~ value t.
-
-Corollary soundness : forall mt m m' t t' T,
-  mt / empty |-- t is T ->
-  well_typed_memory mt m ->
-  m / t -->* m' / t' ->
-  ~ (stuck m' t').
+Theorem progress : forall m mt ths,
+  well_typed_program mt m ths ->
+  (finished ths \/ exists m' ths' ceff, m / ths ==> m' / ths' # ceff).
 Proof.
-  intros * ? ? Hmultistep [Hnormal_form ?]. generalize dependent mt.
-  unfold normal_form in Hnormal_form. induction Hmultistep; intros.
-  - assert (value t \/ exists m' t' eff, m / t --> eff / m' / t') as [? | ?];
-    eauto using progress.
-  - assert (exists mt',
-      mt' extends mt /\
-      mt' / empty |-- t is T /\
-      well_typed_memory mt' m) as [? [? [? ?]]].
-    eauto using preservation.
-    assert (value t \/ exists m' t' eff, m / t --> eff / m' / t') as [? | ?];
-    eauto using progress.
-Qed.
-
-(* ------------------------------------------------------------------------- *)
-(* Concurrent Progress, Preservation & Soundness --------------------------- *)
-(* ------------------------------------------------------------------------- *)
-
-Definition get_ctx := get (@empty typ).
-
-Definition empties (ths : list tm) :=
-  List.repeat (@empty typ) (length ths).
-
-Definition well_typed_threads mt Gammas ths := forall i,
-  exists T, mt / (get_ctx Gammas i) |-- (get_tm ths i) is T.
-
-Definition finished ths :=
-  forall i, value (get_tm ths i).
-
-Lemma empties_length : forall ths,
-  length (empties ths) = length ths.
-Proof.
-  intros. unfold empties. induction ths.
-  - reflexivity.
-  - simpl. f_equal. auto.
-Qed.
-
-Lemma empties_get : forall ths i,
-  get_ctx (empties ths) i = empty.
-Proof.
-  intros *. unfold get_ctx, empties. generalize dependent i.
-  induction ths as [| ? ? IH]; intros i; destruct i; trivial.
-  apply IH.
-Qed.
-
-Lemma empties_set : forall ths i t,
-  empties (set ths i t) = empties ths.
-Proof.
-  intros. unfold empties. rewrite <- set_preserves_length. reflexivity.
-Qed.
-
-Lemma well_typed_threads_destruct : forall mt th ths,
-  well_typed_threads mt (empties (th :: ths)) (th :: ths) ->
-  well_typed_threads mt (empties ths) ths.
-Proof.
-  intros *. intros H i. specialize (H (S i)) as [T H].
-  exists T. unfold get_tm, get_ctx in *. assumption.
-Qed.
-
-Lemma finished_nil : finished nil.
-Proof.
-  intros i. destruct i; apply V_Nil.
-Qed.
-
-Lemma finished_cons : forall th ths,
-  value th ->
-  finished ths ->
-  finished (th :: ths).
-Proof.
-  intros th ths ? ? i. destruct i; unfold get_tm; simpl; trivial.
-Qed.
-
-Lemma cstep_cons : forall m m' th ths ths',
-  m / ths ==> m' / ths' ->
-  m / (th :: ths) ==> m' / (th :: ths').
-Proof.
-  intros * H. destruct H;
-  repeat (
-    try (  eapply CST_None  with (i := S i) (ths := th :: ths)
-        || eapply CST_Spawn with (i := S i) (ths := th :: ths)
-        );
-    simpl; auto using lt_n_S;
-    unfold get_tm; rewrite get_S_i; assumption
-   ).
-Qed.
-
-Lemma step_preserves_thread_typing : forall mt m m' eff ths t i,
-  m / get_tm ths i --> eff / m' / t ->
-  well_typed_memory mt m ->
-  well_typed_threads mt (empties ths) ths ->
-  exists mt',
-    mt' extends mt /\
-    well_typed_threads mt' (empties (set ths i t)) (set ths i t) /\
-    well_typed_memory mt' m'.
-Proof.
-  intros * Hstep Hmem Htypes.
-  destruct (Htypes i) as [T Htype].
-  rewrite empties_get in Htype.
-  assert (exists mt',
-            mt' extends mt /\
-            mt' / empty |-- t is T /\
-            well_typed_memory mt' m') as [? [? [? ?]]].
-  { eauto using preservation. }
-  eexists. splits 3; eauto.
-  intros i'. rewrite empties_get. unfold get_tm.
-  destruct (i =? i') eqn:E.
-  + apply Nat.eqb_eq in E. subst.
-    destruct (le_lt_dec (length ths) i').
-    * rewrite get_set_default; eauto using T_Nil.
-    * rewrite get_set_involutive; eauto.
-  + apply Nat.eqb_neq in E. apply not_eq_sym in E.
-    rewrite get_set_i_neq_j; trivial.
-    destruct (le_lt_dec (length ths) i').
-    * rewrite get_default; eauto using T_Nil.
-    * specialize (Htypes i') as [? ?].
-      unfold get_tm in *. rewrite empties_get in *.
-      eauto using memory_weakening.
-Qed.
-
-Lemma spawn_preserves_thread_typing : forall mt mt' ths block T,
-  mt' extends mt ->
-  mt / empty |-- block is T ->
-  well_typed_threads mt (empties ths) ths ->
-  well_typed_threads mt' (empties (add ths block)) (add ths block).
-Proof.
-  intros * Hext Htype Htypes i.
-  destruct (lt_eq_lt_dec i (length ths)) as [[? | ?] | ?]; unfold get_tm.
-  - specialize (Htypes i) as [T' ?]. exists T'.
-    rewrite get_add_lt; trivial. rewrite empties_get in *.
-    eauto using memory_weakening.
-  - exists T. subst. rewrite get_add_last.
-    rewrite empties_get. eauto using memory_weakening.
-  - rewrite get_add_gt; trivial. rewrite empties_get. eauto using T_Nil.
-Qed.
-
-Lemma spawn_block_has_type: forall mt m m' t t' block T,
-  mt / empty |-- t is T ->
-  m / t --> EF_Spawn block / m' / t' ->
-  exists B, mt / empty |-- block is B.
-Proof.
-  intros ? ? ? t. induction t; intros * Htype Hstep;
-  inversion Hstep; inversion Htype; subst; eauto.
-Qed.
-
-Theorem cpreservation : forall ths ths' m m' mt,
-  well_typed_threads mt (empties ths) ths ->
-  well_typed_memory mt m ->
-  m / ths ==> m' / ths' ->
-  exists mt',
-    mt' extends mt /\
-    well_typed_threads mt' (empties ths') ths' /\
-    well_typed_memory mt' m'.
-Proof.
-  intros * Htypes Hmem Hcstep. induction Hcstep.
-  - eauto using step_preserves_thread_typing.
-  - rewrite add_set_comm; trivial.
-    eapply step_preserves_thread_typing; eauto.
-    + unfold get_tm in *. rewrite get_add_lt; eauto.
-    + destruct (Htypes i) as [T Htype]. rewrite empties_get in Htype.
-      assert (exists B, mt / empty |-- block is B) as [? ?].
-      { eauto using spawn_block_has_type. }
-      eauto using spawn_preserves_thread_typing, extends_refl.
-Qed.
-
-Theorem cprogress : forall ths m mt,
-  well_typed_memory mt m ->
-  well_typed_threads mt (empties ths) ths ->
-  (finished ths \/ exists m' ths', m / ths ==> m' / ths').
-Proof.
-  intros * Hmem Htypes.
+  intros * [Hmem Hths].
   induction ths as [| th ths IH].
-  - left. apply finished_nil.
-  - apply well_typed_threads_destruct in Htypes as Htypes'.
-    specialize (IH Htypes') as [IH | [m' [ths' IH]]].
-    + destruct (is_value th) eqn:E.
-      * left. apply value_equivalence in E. eauto using finished_cons.
-      * right. specialize (Htypes 0) as [T Htype]. rewrite empties_get in Htype.
-        assert (value th \/ exists m' th' eff, m / th --> eff / m' / th')
-        as [F | [m' [th' [eff Hstep]]]].
-        { eauto using progress. }
-        ** apply value_equivalence in F. rewrite E in F. discriminate.
-        ** destruct eff; eauto using cstep, Nat.lt_0_succ.
-    + right. eauto using cstep_cons.
+  - left. intros i. destruct i; auto using value.
+  - destruct (is_value th) eqn:E.
+    + apply value_equivalence_true in E.
+      destruct (IH (well_typed_threads_tail _ _ _ Hths)) as [? | [? [? [? ?]]]].
+      * left. intros i. destruct i; eauto.
+      * right. eexists. eexists. eauto using concurrent_step_weakening.
+    + apply value_equivalence_false in E. right.
+      specialize (IH (well_typed_threads_tail _ _ _ Hths)) as [? | IH].
+      * destruct (Hths 0) as [T Htype].
+        unfold get_tm in Htype. simpl in Htype.
+        assert (value th \/ exists th' eff,
+          th --[eff]--> th' /\
+          well_behaved_effect eff m)
+          as [? | [th' [eff [Hstep Heff]]]];
+        eauto using limited_progress; try contradiction.
+        destruct eff; inversion Heff; subst;
+        eauto using cstep, Nat.lt_0_succ.
+      * specialize IH as [? [? [? ?]]].
+        eexists. eexists. eauto using concurrent_step_weakening.
 Qed.
 
-Definition cnormal_form m th : Prop :=
-  ~ exists m' th', m / th ==> m' / th'.
-
-Definition cstuck m th : Prop := cnormal_form m th /\ ~ finished th.
-
+(*
 Corollary csoundness : forall mt m m' ths ths',
-  well_typed_memory mt m ->
-  well_typed_threads mt (empties ths) ths ->
+  well_typed_program mt m ths ->
   m / ths ==>* m' / ths' ->
   ~ (cstuck m' ths').
 Proof.
-  intros * ? ? Hmultistep [Hnormal_form ?]. generalize dependent mt.
-  unfold cnormal_form in Hnormal_form. induction Hmultistep; intros.
-  - assert (finished ths \/ exists m' ths', m / ths ==> m' / ths') as [? | ?];
-    eauto using cprogress.
-  - assert (exists mt',
-      mt' extends mt /\
-      well_typed_threads mt' (empties ths) ths /\
-      well_typed_memory mt' m) as [? [? [? ?]]].
-    { eauto using cpreservation. }
-    assert (finished ths \/ exists m' ths', m / ths ==> m' / ths') as [? | ?];
-    eauto using cprogress.
 Qed.
+*)
